theories/LambdaCube/Operational.v
@@ -1,0 +1,13 @@
+From Coq Require Import Utf8.
+From FormArith Require Import Base.
+From FormArith.LambdaCube Require Import Term.
+
+Inductive head_step {n : nat} : term n → term n → Prop :=
+| beta_red
+    (ty : term n)
+    (body : term (S n))
+    (arg : term n) : head_step (App (Abs ty body) arg) (bind (bind_first arg) body).
+
+Inductive step {n : nat} : term n → term n → Prop :=
+| ctx_red (K : ctx n) (t u : term n) :
+  head_step t u → step (fill K t) (fill K u).
